WIP

src/Closing.v
@@ -1,34 +1,37 @@
 Require Import String PeanoNat Compare_dec StrictProp.
-Require Import Morph Var.
+Require Import Var.
 
 Definition raw_closing := list (option var).
 
-Definition is_raw_closing_nil (r : raw_closing) :=
+Definition is_pushes_nil (r : list (option var)) :=
   match r with
   | nil => true
   | _ => false
   end.
 
-Fixpoint normalized_raw_closing r :=
+Fixpoint is_normalized_pushes r :=
   match r with
-  | nil => sUnit
+  | nil => true
   | cons vo r =>
-    if andb (var_opt_eqb vo zero_var_opt)
-            (is_raw_closing_nil r)
-    then sEmpty
-    else normalized_raw_closing r
+    if andb (var_opt_eqb vo zero_var_opt) (is_pushes_nil r)
+    then false
+    else is_normalized_pushes r
   end.
 
-Definition normalized_raw_closing_from_cons {r vo} :
-  normalized_raw_closing (cons vo r) ->
-  normalized_raw_closing r.
+Definition normalized_pushes r :=
+  if is_normalized_pushes r then sUnit
+  else sEmpty.
+
+Definition normalized_pushes_from_cons {r vo} :
+  normalized_pushes (cons vo r) ->
+  normalized_pushes r.
 Proof. destruct vo as [[|[]]|], r; easy. Defined.
 
 Set Primitive Projections.
 Record closing :=
   mkclosing {
       c_raw : raw_closing;
-      c_normalized : normalized_raw_closing c_raw
+      c_normalized : normalized_pushes c_raw
     }.
 Add Printing Constructor closing.
 Unset Primitive Projections.
@@ -36,58 +39,81 @@ Unset Primitive Projections.
 Definition closing_id : closing :=
   mkclosing nil stt.
 
-Definition normalized_raw_closing_push0 r vo :=
+Definition normalized_pushes_cons vo r :=
   if andb (var_opt_eqb vo zero_var_opt)
-          (is_raw_closing_nil r)
+          (is_pushes_nil r)
   then nil
   else cons vo r.
 
-Definition normalized_raw_closing_push0_normalized {r vo} :
-  normalized_raw_closing r ->
-  normalized_raw_closing (normalized_raw_closing_push0 r vo).
+Definition normalized_pushes_cons_normalized {vo r} :
+  normalized_pushes r ->
+  normalized_pushes (normalized_pushes_cons vo r).
 Proof. destruct vo as [[|[]]|], r; easy. Defined.
 
-Definition closing_push0 r vo :=
+Definition closing_cons0 vo r :=
   mkclosing
-    (normalized_raw_closing_push0 (c_raw r) vo)
-    (normalized_raw_closing_push0_normalized
+    (normalized_pushes_cons vo (c_raw r))
+    (normalized_pushes_cons_normalized
        (c_normalized r)).
 
 Definition closing_weak0 r :=
-  closing_push0 r None.
+  closing_cons0 None r.
 
 Definition closing_exchange0 r l :=
-  closing_push0 r (Some (bound l)).
+  closing_cons0 (Some (bound l)) r.
 
 Definition closing_close0 r n :=
-  closing_push0 r (Some (free n)).
+  closing_cons0 (Some (free n)) r.
 
-Fixpoint closing_push l r vo :=
-  match l with
-  | 0 => closing_push0 r vo
-  | S l =>
-    match r with
-    | mkclosing nil norm =>
-      closing_push0
-        (closing_push l r (unshift_var_opt zero_var_opt vo))
-        (shift_var_opt vo zero_var_opt)
-    | mkclosing (cons vo' r) norm =>
-      closing_push0
-        (closing_push l
-           (mkclosing r (normalized_raw_closing_from_cons norm))
-           (unshift_var_opt vo' vo))
-        (shift_var_opt vo vo')
-    end
+Definition raw_closing_hd r :=
+  match r with
+  | nil => zero_var_opt
+  | cons vo' _ => vo'
   end.
 
+Definition raw_closing_tl (r : raw_closing) :=
+  match r with
+  | nil => nil
+  | cons _ r' => r'
+  end.
+
+Fixpoint raw_closing_cons l vo r :=
+  match l with
+  | 0 => normalized_pushes_cons vo r
+  | S l =>
+    normalized_pushes_cons
+      (shift_var_opt vo (raw_closing_hd r))
+      (raw_closing_cons
+         l (unshift_var_opt (raw_closing_hd r) vo)
+         (raw_closing_tl r))
+  end.
+
+Definition raw_closing_cons_normalized {l vo r} :
+  normalized_pushes r ->
+  normalized_pushes (raw_closing_cons l vo r).
+Proof.
+  generalize dependent vo.
+  generalize dependent r.
+  induction l; cbn; intros r vo Hnorm;
+    apply normalized_pushes_cons_normalized; try easy.
+  apply IHl.
+  destruct r as [|vo' r]; try easy.
+  apply normalized_pushes_from_cons in Hnorm; easy.
+Defined.
+
+Definition closing_cons l vo r :=
+  mkclosing
+    (raw_closing_cons l vo (c_raw r))
+    (raw_closing_cons_normalized (c_normalized r)).
+
 Definition closing_weak l r :=
-  closing_push l r None.
+  closing_cons l None r.
 
-Definition closing_exchange l1 r l2 :=
-  closing_push l1 r (Some (bound l2)).
+Definition closing_exchange l1 l2 r :=
+  closing_cons l1 (Some (bound l2)) r.
 
-Definition closing_close l r n :=
-  closing_push l r (Some (free n)).
+Definition closing_close l n r :=
+  closing_cons l (Some (free n)) r.
 
 Fixpoint closing_weak_n N : closing :=
   match N with
@@ -98,7 +124,7 @@ Fixpoint closing_weak_n N : closing :=
 Fixpoint closing_weakening N M : closing :=
   match N with
   | 0 => closing_weak_n M
-  | S N => closing_exchange 0 (closing_weakening N M) 0
+  | S N => closing_exchange 0 0 (closing_weakening N M)
   end.
 
 Fixpoint apply_raw_closing_var r : var_op :=
@@ -121,30 +147,30 @@ Add Printing Constructor closing_rhs.
 Unset Primitive Projections.
 
 Definition normalized_closing_rhs r :=
-  normalized_raw_closing (rhs_raw_closing r).
+  normalized_pushes (rhs_raw_closing r).
 
-Definition closing_rhs_push0 r vo :=
+Definition closing_rhs_cons0 vo r :=
   mk_closing_rhs
-    (normalized_raw_closing_push0 (rhs_raw_closing r)
-       (unshift_var_opt (rhs_push r) vo))
+    (normalized_pushes_cons
+       (unshift_var_opt (rhs_push r) vo)
+       (rhs_raw_closing r))
     (shift_var_opt vo (rhs_push r)).
 
 Definition closing_rhs_weak0 r :=
-  closing_rhs_push0 r None.
+  closing_rhs_cons0 None r.
 
-Definition closing_rhs_exchange0 r l :=
-  closing_rhs_push0 r (Some (bound l)).
+Definition closing_rhs_exchange0 l r :=
+  closing_rhs_cons0 (Some (bound l)) r.
 
-Definition closing_rhs_close0 r n :=
-  closing_rhs_push0 r (Some (free n)).
+Definition closing_rhs_close0 n r :=
+  closing_rhs_cons0 (Some (free n)) r.
 
-Definition closing_rhs_push0_normalized {r vo} :
+Definition closing_rhs_cons0_normalized {vo r} :
   normalized_closing_rhs r ->
-  normalized_closing_rhs
-    (closing_rhs_push0 r vo).
+  normalized_closing_rhs (closing_rhs_cons0 vo r).
 Proof.
   destruct r as [? []]; cbn;
-    apply normalized_raw_closing_push0_normalized;
+    apply normalized_pushes_cons_normalized;
     easy.
 Defined.
 
@@ -153,22 +179,21 @@ Fixpoint transpose_push_raw_closing vo r {struct r} :=
   | nil => mk_closing_rhs nil vo
   | cons vo' r =>
     if var_opt_eqb vo zero_var_opt then mk_closing_rhs r vo'
-    else closing_rhs_push0
+    else closing_rhs_cons0 vo'
            (transpose_push_raw_closing
               (unshift_var_var_opt zero_var vo) r)
-           vo'
   end.
 
 Definition transpose_push_raw_closing_normalized {vo r} :
-  normalized_raw_closing r ->
+  normalized_pushes r ->
   normalized_closing_rhs
     (transpose_push_raw_closing vo r).
 Proof.
   generalize dependent vo.
   induction r as [|vo' r]; intros vo norm; try easy; cbn.
-  apply normalized_raw_closing_from_cons in norm.
+  apply normalized_pushes_from_cons in norm.
   destruct (var_opt_eqb vo zero_var_opt); try easy.
-  apply closing_rhs_push0_normalized.
+  apply closing_rhs_cons0_normalized.
   apply IHr; easy.
 Defined.
 
@@ -177,20 +202,20 @@ Fixpoint compose_raw_closing r1 r2 :=
   | nil => r2
   | cons vo r1 =>
     let rhs := transpose_push_raw_closing vo r2 in
-    normalized_raw_closing_push0
-      (compose_raw_closing r1 (rhs_raw_closing rhs))
+    normalized_pushes_cons
       (rhs_push rhs)
+      (compose_raw_closing r1 (rhs_raw_closing rhs))
   end.
 
 Definition compose_raw_closing_normalized {r1 r2} :
-  normalized_raw_closing r1 ->
-  normalized_raw_closing r2 ->
-  normalized_raw_closing (compose_raw_closing r1 r2).
+  normalized_pushes r1 ->
+  normalized_pushes r2 ->
+  normalized_pushes (compose_raw_closing r1 r2).
 Proof.
   generalize dependent r2.
   induction r1 as [|vo]; intros r2 norm1 norm2; try easy.
-  apply normalized_raw_closing_from_cons in norm1; cbn.
-  apply normalized_raw_closing_push0_normalized.
+  apply normalized_pushes_from_cons in norm1; cbn.
+  apply normalized_pushes_cons_normalized.
   apply IHr1; try easy.
   apply transpose_push_raw_closing_normalized; easy.
 Defined.
