src/Label.v
@@ -1,0 +1,66 @@
+Require Import Ascii String StrictProp.
+
+Definition label := string.
+
+Definition label_dec s1 s2 := string_dec s1 s2.
+Arguments label_dec !s1 !s2.
+
+Definition is_less_than_ascii (a1 : ascii) (a2 : ascii) :=
+  match a1, a2 with
+  | Ascii b11 b12 b13 b14 b15 b16 b17 b18,
+    Ascii b21 b22 b23 b24 b25 b26 b27 b28 =>
+    match b18, b28 with
+    | true, false => false
+    | false, true => true
+    | _, _ =>
+      match b17, b27 with
+      | true, false => false
+      | false, true => true
+      | _, _ =>
+        match b16, b26 with
+        | true, false => false
+        | false, true => true
+        | _, _ =>
+          match b15, b25 with
+          | true, false => false
+          | false, true => true
+          | _, _ =>
+            match b14, b24 with
+            | true, false => false
+            | false, true => true
+            | _, _ =>
+              match b13, b23 with
+              | true, false => false
+              | false, true => true
+              | _, _ =>
+                match b12, b22 with
+                | true, false => false
+                | false, true => true
+                | _, _ =>
+                  match b11, b21 with
+                  | true, false => false
+                  | false, true => true
+                  | _, _ => false
+                  end
+                end
+              end
+            end
+          end
+        end
+      end
+    end
+  end.
+
+Fixpoint is_less_than_label s1 s2 :=
+  match s1, s2 with
+  | EmptyString, EmptyString => false
+  | String a1 s1, EmptyString => false
+  | EmptyString, String a2 s2 => true
+  | String a1 s1, String a2 s2 =>
+    if is_less_than_ascii a1 a2 then true
+    else if is_less_than_ascii a2 a1 then false
+    else is_less_than_label s1 s2
+  end.
+
+Definition less_than_label s1 s2 :=
+  if is_less_than_label s1 s2 then sUnit else sEmpty.
