src/Renaming.v
@@ -1,412 +1,61 @@
-Require Import String PeanoNat Compare_dec StrictProp.
-Require Import Morph Var.
+Require Import Label PeanoNat Compare_dec StrictProp.
+Require Import Var Closing.
 
-Inductive renaming (N : nat) : nat -> Set :=
-| renaming_closing : forall M, closing N M -> renaming N M
-| renaming_shift : forall M,
-    name -> renaming N M -> renaming N M
-| renaming_open : forall M,
-    name -> renaming N M -> level (S M) ->
-    renaming N (S M)
-| renaming_rename : forall M,
-    name -> renaming N M -> name -> renaming N M.
+Definition raw_renaming_pushes : Type :=
+  list (label * list (option var)).
 
-Arguments renaming_closing {N} {M} r.
-Arguments renaming_shift {N} {M} n r.
-Arguments renaming_open {N} {M} n r l.
-Arguments renaming_rename {N} {M} n1 r n2.
-
-Definition renaming_nil :=
-  renaming_closing closing_nil.
-
-Definition renaming_id {N} : renaming N N :=
-  renaming_closing closing_id.
-
-Fixpoint renaming_zero_weak {N M} (r : renaming N M) :
-  renaming (S N) M :=
-  match r in renaming _ M
-        return renaming _ M
-  with
-  | renaming_closing r =>
-    renaming_closing (closing_zero_weak r)
-  | renaming_shift n r =>
-    renaming_shift n (renaming_zero_weak r)
-  | @renaming_open _ M n r l =>
-    renaming_open n (renaming_zero_weak r) l
-  | renaming_rename n1 r n2 =>
-    renaming_rename n1 (renaming_zero_weak r) n2
+Definition is_less_than_renaming_pushes
+           s (r : raw_renaming_pushes) :=
+  match r with
+  | nil => true
+  | cons (s', ps) r => is_less_than_label s s'
   end.
 
-Fixpoint renaming_weak {N M}
-         (l : level (S N)) (r : renaming N M) :
-  renaming (S N) M :=
-  match r in renaming _ M
-        return renaming _ M
-  with
-  | renaming_closing r =>
-    renaming_closing (closing_weak l r)
-  | renaming_shift n r =>
-    renaming_shift n (renaming_weak l r)
-  | @renaming_open _ M n r l' =>
-    renaming_open n (renaming_weak l r) l'
-  | renaming_rename n1 r n2 =>
-    renaming_rename n1 (renaming_weak l r) n2
+Fixpoint is_normalized_raw_renaming_pushes
+         (r : raw_renaming_pushes) :=
+  match r with
+  | nil => true
+  | cons (s, ps) r =>
+    andb
+      (is_less_than_renaming_pushes s r)
+      (andb
+         (andb (negb (is_pushes_nil ps))
+               (is_normalized_pushes ps))
+         (is_normalized_raw_renaming_pushes r))
   end.
 
-Fixpoint renaming_zero_exchange {N M}
-         (r : renaming N M) :
-  level (S M) -> renaming (S N) (S M) :=
-  match r in renaming _ M
-        return level (S M) -> renaming _ (S M)
-  with
-  | renaming_closing r =>
-    fun l2 => renaming_closing (closing_zero_exchange r l2)
-  | renaming_shift n r =>
-    fun l2 => renaming_shift n (renaming_zero_exchange r l2)
-  | @renaming_open _ M n r l =>
-    fun l2 =>
-      renaming_open
-        n (renaming_zero_exchange r
-             (@unshift_level (S (S M)) l l2))
-        (shift_level l2 l)
-  | renaming_rename n1 r n2 =>
-    fun l2 =>
-      renaming_rename n1 (renaming_zero_exchange r l2) n2
-  end.
+Definition normalized_raw_renaming_pushes r :=
+  if is_normalized_raw_renaming_pushes r then sUnit
+  else sEmpty.
 
-Fixpoint renaming_exchange {N M}
-         (l1 : level (S N)) (r : renaming N M) :
-  level (S M) -> renaming (S N) (S M) :=
-  match r in renaming _ M
-        return level (S M) -> renaming _ (S M)
-  with
-  | renaming_closing r =>
-    fun l2 => renaming_closing (closing_exchange l1 r l2)
-  | renaming_shift n r =>
-    fun l2 => renaming_shift n (renaming_exchange l1 r l2)
-  | @renaming_open _ M n r l =>
-    fun l2 =>
-      renaming_open
-        n (renaming_exchange l1 r
-             (@unshift_level (S (S M)) l l2))
-        (shift_level l2 l)
-  | renaming_rename n1 r n2 =>
-    fun l2 =>
-      renaming_rename n1 (renaming_exchange l1 r l2) n2
-  end.
+Set Primitive Projections.
+Record raw_renaming :=
+  mk_raw_renaming {
+      r_renaming : raw_renaming_pushes;
+      r_closing : raw_closing;
+    }.
+Add Printing Constructor raw_renaming.
+Unset Primitive Projections.
 
-Fixpoint renaming_zero_close {N M}
-         (r : renaming N M) (n : name) :
-  renaming (S N) M :=
-  match r in renaming _ M
-        return renaming _ M
-  with
-  | renaming_closing r =>
-    renaming_closing (closing_zero_close r n)
-  | renaming_shift n' r =>
-    renaming_shift n' (renaming_zero_close r n)
-  | @renaming_open _ M n' r l' =>
-    renaming_open n' (renaming_zero_close r n) l'
-  | renaming_rename n1 r n2 =>
-    renaming_rename
-      n1 (renaming_zero_close r (unshift_name n2 n))
-      (shift_name n n2)
-  end.
+Definition is_normalized_raw_renaming r :=
+  andb (is_normalized_raw_renaming_pushes (r_renaming r))
+       (is_normalized_pushes (r_closing r)).
 
-Fixpoint renaming_close {N M}
-         (l : level (S N)) (r : renaming N M) (n : name) :
-  renaming (S N) M :=
-  match r in renaming _ M
-        return renaming _ M
-  with
-  | renaming_closing r =>
-    renaming_closing (closing_close l r n)
-  | renaming_shift n' r =>
-    renaming_shift n' (renaming_close l r n)
-  | @renaming_open _ M n' r l' =>
-    renaming_open n' (renaming_close l r n) l'
-  | renaming_rename n1 r n2 =>
-    renaming_rename
-      n1 (renaming_close l r (unshift_name n2 n))
-      (shift_name n n2)
-  end.
+Definition normalized_raw_renaming r :=
+  if is_normalized_raw_renaming r then sUnit
+  else sEmpty.
 
-Fixpoint apply_renaming_var {N M}
-         (r : renaming N M)
-  : morph var M var N :=
-  match r in renaming _ M
-        return morph _ M _ _ with
-  | renaming_closing r => apply_closing_var r
-  | @renaming_shift _ M n r =>
-      morph_extend_by N (@open_var n)
-      @ lift_morph_var (apply_renaming_var r)
-      @ morph_extend_by M (@weak_var)
-  | @renaming_open _ M n r l =>
-      morph_extend_by N (@open_var n)
-      @ lift_morph_var (apply_renaming_var r)
-      @ @cycle_in_var (S M) l
-  | @renaming_rename _ M n1 r n2 =>
-      morph_extend_by N (@open_var n1)
-      @ lift_morph_var (apply_renaming_var r)
-      @ morph_extend_by M (@close_var n2)
-  end.
+Set Primitive Projections.
+Record renaming :=
+  mk_renaming {
+      r_raw : raw_renaming;
+      r_normalized : normalized_raw_renaming r_raw;
+    }.
+Add Printing Constructor renaming.
+Unset Primitive Projections.
 
-Inductive renaming_rhs (N : nat) : nat -> Set :=
-| renaming_rhs_shift_rhs : forall M,
-    renaming N M -> renaming_rhs N M
-| renaming_rhs_open_rhs : forall M,
-    renaming N M -> level (S M) ->
-    renaming_rhs N (S M)
-| renaming_rhs_rename_rhs : forall M,
-    renaming N M -> name ->
-    renaming_rhs N M.
 
-Arguments renaming_rhs_shift_rhs {N} {M} r.
-Arguments renaming_rhs_open_rhs {N} {M} r l.
-Arguments renaming_rhs_rename_rhs {N} {M} r n.
 
-Definition renaming_rhs_shift {N M}
-          n1 (r : renaming_rhs N M)
-  : renaming_rhs N M :=
-  match r in renaming_rhs _ M
-        return renaming_rhs _ M with
-  | renaming_rhs_shift_rhs r =>
-      renaming_rhs_shift_rhs
-        (renaming_shift n1 r)
-  | renaming_rhs_open_rhs r l =>
-      renaming_rhs_open_rhs
-        (renaming_shift n1 r) l
-  | renaming_rhs_rename_rhs r n =>
-      renaming_rhs_rename_rhs
-        (renaming_shift n1 r) n
-  end.
 
-Definition renaming_rhs_open {N M}
-           n1 (r : renaming_rhs N M)
-  : level (S M) -> renaming_rhs N (S M) :=
-  match r in renaming_rhs _ M
-        return level (S M) ->
-               renaming_rhs _ (S M)
-  with
-  | renaming_rhs_shift_rhs r =>
-    fun l1 =>
-      renaming_rhs_shift_rhs
-        (renaming_open n1 r l1)
-  | @renaming_rhs_open_rhs _ M' r l =>
-    fun l1 =>
-      renaming_rhs_open_rhs
-        (renaming_open n1 r (@unshift_level (S (S M')) l l1))
-        (shift_level l1 l)
-  | renaming_rhs_rename_rhs r n =>
-    fun l1 =>
-      renaming_rhs_rename_rhs
-        (renaming_open n1 r l1) n
-  end.
 
-Definition renaming_rhs_rename {N M}
-           n1 (r : renaming_rhs N M) n2
-  : renaming_rhs N M :=
-  match r in renaming_rhs _ M
-        return renaming_rhs _ M
-  with
-  | renaming_rhs_shift_rhs r =>
-    renaming_rhs_shift_rhs
-      (renaming_rename n1 r n2)
-  | renaming_rhs_open_rhs r l =>
-    renaming_rhs_open_rhs
-      (renaming_rename n1 r n2) l
-  | renaming_rhs_rename_rhs r n =>
-    renaming_rhs_rename_rhs
-      (renaming_rename n1 r (unshift_name n n2))
-      (shift_name n2 n)
-  end.
 
-Fixpoint transpose_level_renaming {N M}
-         l (r : renaming N M)
-  : renaming_rhs (pred N) M :=
-  match r in renaming _ M
-        return renaming_rhs _ M
-  with
-  | renaming_closing r =>
-      match transpose_level_closing r l
-            in closing_rhs _ M'
-            return renaming_rhs _ M'
-      with
-      | closing_rhs_weak_rhs r =>
-        renaming_rhs_shift_rhs
-          (renaming_closing r)
-      | closing_rhs_exchange_rhs r l =>
-        renaming_rhs_open_rhs
-          (renaming_closing r) l
-      | closing_rhs_close_rhs r n =>
-        renaming_rhs_rename_rhs
-          (renaming_closing r) n
-      end
-  | renaming_shift n1 r =>
-      renaming_rhs_shift n1
-        (transpose_level_renaming l r)
-  | renaming_open n1 r l2 =>
-      renaming_rhs_open
-        n1 (transpose_level_renaming l r) l2
-  | renaming_rename n1 r n2 =>
-      renaming_rhs_rename
-        n1 (transpose_level_renaming l r) n2
-  end.
-
-Fixpoint transpose_name_renaming {N M}
-         n (r : renaming N M)
-  : renaming_rhs N M :=
-  match r in renaming _ M
-        return renaming_rhs _ M
-  with
-  | renaming_closing r =>
-    match transpose_name_closing r n
-          in closing_rhs _ M'
-          return renaming_rhs _ M'
-    with
-    | closing_rhs_weak_rhs r =>
-      renaming_rhs_shift_rhs
-        (renaming_closing r)
-    | closing_rhs_exchange_rhs r l =>
-      renaming_rhs_open_rhs
-        (renaming_closing r) l
-    | closing_rhs_close_rhs r n =>
-      renaming_rhs_rename_rhs
-        (renaming_closing r) n
-    end
-  | renaming_shift n1 r =>
-    if name_eqb n n1 then
-      renaming_rhs_shift_rhs r
-    else
-      renaming_rhs_shift
-        (unshift_name n n1)
-        (transpose_name_renaming (unshift_name n1 n) r)
-  | renaming_open n1 r l2 =>
-    if name_eqb n n1 then
-      renaming_rhs_open_rhs r l2
-    else
-      renaming_rhs_open
-        (unshift_name n n1)
-        (transpose_name_renaming (unshift_name n1 n) r) l2
-  | renaming_rename n1 r n2 =>
-    if name_eqb n n1 then
-      renaming_rhs_rename_rhs r n2
-    else
-      renaming_rhs_rename
-        (unshift_name n n1)
-        (transpose_name_renaming (unshift_name n1 n) r) n2
-  end.
-
-Fixpoint compose_closing_renaming {N M O}
-         (r1 : closing O N) {struct r1}
-  : renaming N M -> renaming O M :=
-  match r1 in closing O' N'
-        return renaming N' _ -> renaming O' _
-  with
-  | closing_nil => fun r2 => r2
-  | closing_zero_weak r1 =>
-    fun r2 =>
-      renaming_zero_weak
-        (compose_closing_renaming r1 r2)
-  | closing_zero_exchange r1 l2 =>
-    fun r2 =>
-      match transpose_level_renaming l2 r2
-             in renaming_rhs _ M
-             return renaming _ M
-      with
-      | renaming_rhs_shift_rhs r2 =>
-          renaming_zero_weak
-            (compose_closing_renaming r1 r2)
-      | renaming_rhs_open_rhs r2 l2 =>
-          renaming_zero_exchange
-            (compose_closing_renaming r1 r2) l2
-      | renaming_rhs_rename_rhs r2 n =>
-          renaming_zero_close
-            (compose_closing_renaming r1 r2) n
-      end
-  | closing_zero_close r1 n =>
-    fun r2 =>
-      match transpose_name_renaming n r2
-            in renaming_rhs _ M
-            return renaming _ M
-       with
-      | renaming_rhs_shift_rhs r2 =>
-          renaming_zero_weak
-            (compose_closing_renaming r1 r2)
-      | renaming_rhs_open_rhs r2 l2 =>
-          renaming_zero_exchange
-            (compose_closing_renaming r1 r2) l2
-      | renaming_rhs_rename_rhs r2 n =>
-          renaming_zero_close
-            (compose_closing_renaming r1 r2) n
-      end
-  end.
-
-Fixpoint compose_renamings {N M O} (r1 : renaming O N) {struct r1}
-  : renaming N M -> renaming O M :=
-  match r1 in renaming _ N'
-        return renaming N' _ -> _
-  with
-  | renaming_closing r1 =>
-    fun r2 =>
-      compose_closing_renaming r1 r2
-  | renaming_shift n r1 =>
-    fun r2 =>
-      renaming_shift n (compose_renamings r1 r2)
-  | renaming_open n r1 l =>
-    fun r2 =>
-      match transpose_level_renaming l r2
-             in renaming_rhs _ M
-             return renaming _ M
-      with
-      | renaming_rhs_shift_rhs r2 =>
-          renaming_shift
-            n (compose_renamings r1 r2)
-      | renaming_rhs_open_rhs r2 l2 =>
-          renaming_open
-            n (compose_renamings r1 r2) l2
-      | renaming_rhs_rename_rhs r2 n2 =>
-          renaming_rename
-            n (compose_renamings r1 r2) n2
-      end
-  | renaming_rename n1 r1 n2 =>
-    fun r2 =>
-      match transpose_name_renaming n2 r2
-            in renaming_rhs _ M
-            return renaming _ M
-       with
-      | renaming_rhs_shift_rhs r2 =>
-          renaming_shift
-            n1 (compose_renamings r1 r2)
-      | renaming_rhs_open_rhs r2 l =>
-          renaming_open
-            n1 (compose_renamings r1 r2) l
-      | renaming_rhs_rename_rhs r2 n3 =>
-          renaming_rename
-            n1 (compose_renamings r1 r2) n3
-      end
-  end.
-
-(*
-
-Declare Scope ren_scope.
-Delimit Scope ren_scope with ren.
-
-Notation "r ; ^ a" := (r_shift a r)
-  (at level 47, left associativity) : ren_scope.
-Notation "r ; a <- b" := (r_rename a r b)
-  (at level 47, left associativity, a at next level)
-  : ren_scope.
-Notation "r ; u // a" := (r_subst u r a)
-  (at level 47, left associativity, u at next level)
-  : ren_scope.
-Notation "r ; a" := (r_rename a r a)
-  (at level 47, left associativity) : ren_scope.
-Notation "^ a" := (r_shift a r_id)
-  (at level 47, left associativity) : ren_scope.
-Notation "a <- b" := (r_rename a r_id b)
-  (at level 47, left associativity) : ren_scope.
-Notation "u // a" := (r_subst u r_id a)
-  (at level 47, left associativity) : ren_scope.
-
-*)
